theories/ordinals/Ackermann/PAtheory.v
@@ -68,7 +68,7 @@ Proof.
                (fun (m : nat) (_ : {0 = m} + {0 <> m}) => 
                   right (0 = S m) (O_S m)) nv) as [a | b1].
           ** elim b; auto.
-          ** fold var ; fold (Succ (var nv)).
+          ** fold (Succ (var nv)).
              apply sysWeaken;  apply existI with (var 0).
              rewrite (subFormulaEqual LNT).
              simpl in |- *.
@@ -159,7 +159,7 @@ Proof.
                      fold
                        (Succ
                           (apply LNT Languages.Plus
-                             (Tcons LNT 1 (fol.var LNT 1) 
+                             (Tcons LNT 1 (var 1) 
                                 (Tcons LNT 0 Zero (Tnil LNT))))) 
                        in |- *.
                      apply eqSucc.
@@ -177,7 +177,7 @@ Proof.
                      fold
                        (Succ
                           (apply LNT Languages.Plus
-                             (Tcons LNT 1 (fol.var LNT 1)
+                             (Tcons LNT 1 (var 1)
                                 (Tcons LNT 0 (Succ (var 0)) (Tnil LNT)))))
                        in |- *.
                      apply eqSucc.
@@ -219,7 +219,7 @@ Proof.
   - apply closedPA.
   - rewrite translateLT1.
     set (nv := newVar (0 :: 2 :: 1 :: 0 :: nil)) in *.
-    fold var; fold Zero; fold (Succ (var nv)); 
+     fold Zero; fold (Succ (var nv)); 
       fold (Plus (var 0) (Succ (var nv))) in |- *.
     apply nnI, forallI.
     + apply closedPA.
@@ -236,11 +236,11 @@ Proof.
   replace (LNN2LNT_formula NN8) with
     (forallH 1
        (forallH 0
-          (impH (LNN2LNT_formula (LNN.LT (LNN.var 0) (LNN.Succ (LNN.var 1))))
-             (orH (LNN2LNT_formula (LNN.LT (LNN.var 0) (LNN.var 1)))
+          (impH (LNN2LNT_formula (LNN.LT (var 0) (LNN.Succ (var 1))))
+             (orH (LNN2LNT_formula (LNN.LT (var 0) (var 1)))
                 (equal (var 0) (var 1)))))); simpl.
   - repeat rewrite translateLT1; simpl.
-    unfold newVar; simpl; fold var; fold (Succ (var 3)).
+    unfold newVar; simpl; fold (Succ (var 3)).
     fold (Succ (var 1)); fold (Plus (var 0) (Succ (var 3))).
     fold (existH 3 (equal (Plus (var 0) (Succ (var 3))) 
                               (Succ (var 1)))).
@@ -315,16 +315,15 @@ Proof.
   replace (LNN2LNT_formula NN9) with
     (forallH 1
        (forallH 0
-          (orH (LNN2LNT_formula (LNN.LT (LNN.var 0) (LNN.var 1)))
+          (orH (LNN2LNT_formula (LNN.LT (var 0) (var 1)))
              (orH (equal (var 0) (var 1))
-                (LNN2LNT_formula (LNN.LT (LNN.var 1) (LNN.var 0)))))));
+                (LNN2LNT_formula (LNN.LT (var 1) (var 0)))))));
     [ idtac | reflexivity ].
   simpl in |- *.
   repeat rewrite translateLT1.
   simpl in |- *.
   unfold newVar in |- *.
   simpl in |- *.
-  fold var in |- *.
   fold (Succ (var 3)) in |- *.
   fold (Plus (var 0) (Succ (var 3))) in |- *.
   fold (Plus (var 1) (Succ (var 3))) in |- *.
@@ -575,7 +574,7 @@ Proof.
                  apply eqSucc.
                  apply sysWeaken.
                  apply pa3.
-                 fold (Succ (fol.var LNT 0)) in |- *.
+                 fold (Succ (var 0)) in |- *.
                  apply eqSucc.
                  apply eqSym.
                  apply Axm; right; constructor.
@@ -608,7 +607,7 @@ Proof.
                  apply eqTrans with (Succ (Plus (Succ (var 1)) (Succ (var 3)))).
                  apply sysWeaken.
                  apply pa4 with (a := Succ (var 1)) (b := Succ (var 3)).
-                 fold (Succ (fol.var LNT 0)) in |- *.
+                 fold (Succ (var 0)) in |- *.
                  apply eqSucc.
                  apply Axm; right; constructor.
 Qed.
