theories/ordinals/Ackermann/fol.v
@@ -721,4 +721,5 @@ Arguments andH {L} _ _.
 Arguments iffH {L} _ _.
 Arguments equal {L} _ _.
 Arguments existH {L} _ _.
+Arguments var {L} _.
 
